upgraded imp

theories/Imp.v
@@ -43,9 +43,25 @@ Set Implicit Arguments.
 (** Imp manipulates a countable set of variables represented as [string]s: *)
 Definition var : Set := string.
 
+(** Imp types *)
+Inductive type : Type :=
+| Tint : type
+| Tptr : type -> type
+.
+
+Definition has_type (v: val) (t: type) : bool :=
+  match v, t with
+  | Vint _, Tint => true
+  | Vptr _ _, Tptr _ => true
+  | Vundef, _ => true
+  | _, _ => false
+  end
+.
+
 Inductive fun_type : Type :=
-| Fun (_ : gname)
-| Sys (_ : gname).
+| Fun (_ : gname) (_ : type)
+| Sys (_ : gname) (_ : type)
+.
 
 (** Expressions are made of variables, constant literals, and arithmetic operations. *)
 Inductive expr : Type :=
@@ -53,9 +69,10 @@ Inductive expr : Type :=
 | Lit (_ : val)
 | Plus  (_ _ : expr)
 | Minus (_ _ : expr)
-| Mult  (_ _ : expr).
+| Mult  (_ _ : expr)
+.
 
-(** LDJ: function call exists only as a statement *)
+(** function call exists only as a statement *)
 Inductive stmt : Type :=
 | Assign (x : var) (e : expr)    (* x = e *)
 | Seq    (a b : stmt)            (* a ; b *)
@@ -63,15 +80,16 @@ Inductive stmt : Type :=
 | While  (t : expr) (b : stmt)   (* while (t) { b } *)
 | Skip                           (* ; *)
 | CallFun (x : var) (f : fun_type) (args : list expr)  (* x = f(args) *)
-| Expr (e : expr)    (* evaluates expression, will be returned if the last stmt *)
+| Return (e : expr)    (* return e *)
 .
 
-(** LDJ: information of a function, maybe add return type? *)
-Record function : Type :=
-  mk_function { params : list var ; body : stmt }.
-
-(** LDJ: a program is a list of (function name, body) *)
-Definition program : Type := list (gname * function).
+(** information of a function *)
+Record function : Type := mk_function {
+  fn_return : type;
+  fn_params : list (var * type);
+  fn_vars : list (var * type); (* includes fn_params *)
+  fn_body : stmt
+}.
 
 (* ========================================================================== *)
 (** ** Notations *)
@@ -79,11 +97,11 @@ Definition program : Type := list (gname * function).
 Module ImpNotations.
 
   (** A few notations for convenience.  *)
-  Definition Expr_coerce: expr -> stmt := Expr.
+  Definition Return_coerce: expr -> stmt := Return.
   Definition Var_coerce: string -> expr := Var.
   Definition Lit_coerce: val -> expr := Lit.
   Definition Vint_coerce: Z -> val := Vint.
-  Coercion Expr_coerce: expr >-> stmt.
+  Coercion Return_coerce: expr >-> stmt.
   Coercion Var_coerce: string >-> expr.
   Coercion Lit_coerce: val >-> expr.
   Coercion Vint_coerce: Z >-> val.
@@ -130,37 +148,20 @@ Import ImpNotations.
 (* ========================================================================== *)
 (** ** Semantics *)
 
-(** _Imp_ produces effects by manipulating its variables.  To account for this,
-    we define a type of _external interactions_ [ImpState] modeling reads and
-    writes to global variables.
-
-    A read, [GetVar], takes a variable as an argument and expects the
-    environment to answer with a value, hence defining an event of type
-    [ImpState value].
-
-    Similarly, [SetVar] is a write event parameterized by both a variable and a
-    value to be written, and defines an event of type [ImpState unit], no
-    informative answer being expected from the environment.  *)
+(** Get/Set function local variables *)
 Variant ImpState : Type -> Type :=
 | GetVar (x : var) : ImpState val
 | SetVar (x : var) (v : val) : ImpState unit.
 
 Section Denote.
-
-  (** We now proceed to denote _Imp_ expressions and statements.
-      We could simply fix in stone the universe of events to be considered,
-      taking as a semantic domain for _Imp_ [itree ImpState X]. That would be
-      sufficient to give meaning to _Imp_, but would prohibit us from relating this
-      meaning to [itree]s stemmed from other entities. Therefore, we
-      parameterize the denotation of _Imp_ by a larger universe of events [eff],
-      of which [ImpState] is assumed to be a subevent. *)
-
+ 
   Context `{Σ: GRA.t}.
   Context {eff : Type -> Type}.
   Context {HasImpState : ImpState -< eff}.
   Context {HasCall : callE -< eff}.
   Context {HasEvent : eventE -< eff}.
 
+  (** Denotation of expressions *)
   Fixpoint denote_expr (e : expr) : itree eff val :=
     match e with
     | Var v     => trigger (GetVar v)
@@ -170,6 +171,7 @@ Section Denote.
     | Mult a b  => l <- denote_expr a ;; r <- denote_expr b ;; (vmul l r)?
     end.
 
+  (** Rewriting lemmas *)
   Lemma denote_expr_Var
         v
     :
@@ -203,39 +205,11 @@ Section Denote.
       l <- denote_expr a ;; r <- denote_expr b ;; (vmul l r)?.
   Proof. reflexivity. Qed.
 
-  (** We turn to the denotation of statements. As opposed to expressions,
-      statements do not return any value: their semantic domain is therefore
-      [itree eff unit]. The most interesting construct is, naturally, [while].
-
-      To define its meaning, we make use of the [iter] combinator provided by
-      the [itree] library:
-
-      [iter : (A -> itree E (A + B)) -> A -> itree E B].
-
-      The combinator takes as argument the body of the loop, i.e. a function
-      that maps inputs of type [A], the accumulator, to an [itree] computing
-      either a new [A] that can be fed back to the loop, or a return value of
-      type [B]. The combinator builds the fixpoint of the body, hiding away the
-      [A] argument from the return type.
-
-      Compared to the [mrec] and [rec] combinators introduced in
-      [Introduction.v], [iter] is more restricted in that it naturally
-      represents tail recursive functions.  It, however, enjoys a rich equational
-      theory: its addition grants the type of _continuation trees_ (named
-      [ktree]s in the library), a structure of _traced monoidal category_.
-
-      We use [loop] to first build a new combinator [while].
-      The accumulator degenerates to a single [unit] value indicating
-      whether we entered the body of the while loop or not. Since the
-      the operation does not return any value, the return type is also
-      taken to be [unit].
-      That is, the right tag [inr tt] says to exit the loop,
-      while the [inl tt] says to continue. *)
-
+  (** Denotation of statements *)
   Definition while (step : itree eff (unit + val)) : itree eff val :=
     ITree.iter (fun _ => step) tt.
 
-  (** Casting values into [bool]: [Vint 0] corresponds to [false] and any nonzero
+  (** Casting values into [bool]: [Vint 0] corresponds to [false] and any other
       value corresponds to [true].  *)
   Definition is_true (v : val) : option bool :=
     match v with
@@ -243,12 +217,6 @@ Section Denote.
     | _ => None
     end.
 
-  (** The meaning of Imp statements is now easy to define. They are all
-      straightforward, except for [While], which uses our new [while] combinator
-      over the computation that evaluates the conditional, and then the body if
-      the former was true.  *)
-
-  (* change to "v <- ccall f eval_args ;;" ? *)
   Fixpoint denote_stmt (s : stmt) : itree eff val :=
     match s with
     | Assign x e =>  v <- denote_expr e ;; trigger (SetVar x v) ;; Ret Vundef
@@ -265,19 +233,24 @@ Section Denote.
     | Skip => Ret Vundef
     | CallFun x ft args =>
       match ft with
-      | Fun f =>
+      | Fun f ty =>
         eval_args <- (mapT denote_expr args) ;;
         v <- trigger (Call f (eval_args↑)) ;; v <- unwrapN (v↓);;
-        trigger (SetVar x v) ;; Ret Vundef
-      | Sys f =>
+        if (has_type v ty)
+        then trigger (SetVar x v) ;; Ret Vundef
+        else triggerNB
+      | Sys f ty =>
         eval_args <- (mapT denote_expr args) ;;
         v <- trigger (Syscall f eval_args top1) ;;
-        trigger (SetVar x v) ;; Ret Vundef
+        if (has_type v ty)
+        then trigger (SetVar x v) ;; Ret Vundef
+        else triggerNB
       end
 
-    | Expr e => v <- denote_expr e ;; Ret v
+    | Return e => v <- denote_expr e ;; Ret v
     end.
 
+  (** Rewriting lemmas *)
   Lemma denote_stmt_Assign
         x e
     :
@@ -318,21 +291,25 @@ Section Denote.
     :
       denote_stmt (CallFun x ft args) =
       match ft with
-      | Fun f =>
+      | Fun f ty =>
         eval_args <- (mapT denote_expr args) ;;
         v <- trigger (Call f (eval_args↑)) ;; v <- unwrapN (v↓);;
-        trigger (SetVar x v) ;; Ret Vundef
-      | Sys f =>
+        if (has_type v ty)
+        then trigger (SetVar x v) ;; Ret Vundef
+        else triggerNB
+      | Sys f ty =>
         eval_args <- (mapT denote_expr args) ;;
         v <- trigger (Syscall f eval_args top1) ;;
-        trigger (SetVar x v) ;; Ret Vundef
+        if (has_type v ty)
+        then trigger (SetVar x v) ;; Ret Vundef
+        else triggerNB
       end.
   Proof. reflexivity. Qed.
 
-  Lemma denote_stmt_Expr
+  Lemma denote_stmt_Return
         e
     :
-      denote_stmt (Expr e) = v <- denote_expr e ;; Ret v.
+      denote_stmt (Return e) = v <- denote_expr e ;; Ret v.
   Proof. reflexivity. Qed.
 
 End Denote.
@@ -365,114 +342,95 @@ Proof.
 Qed.
 (* end hide *)
 
-(* Definition handle_ImpState {E: Type -> Type} `{mapE var (Vundef) -< E}: ImpState ~> itree E := *)
-(*   fun _ e => *)
-(*     match e with *)
-(*     | GetVar x => lookup_def x *)
-(*     | SetVar x v => insert x v *)
-(*     end. *)
-(* (** We now concretely implement this environment using ExtLib's finite maps. *) *)
-(* Definition lenv := alist var val. *)
-
-Definition lenv := alist var val.
+(** function local environment, local variables included when called *)
+Definition lenv := alist var (type * val).
 Definition handle_ImpState {E: Type -> Type} `{Σ: GRA.t} `{eventE -< E}: ImpState ~> stateT lenv (itree E) :=
-  fun _ e old =>
+  fun _ e le =>
     match e with
-    | GetVar x => r <- unwrapU (alist_find _ x old) ;; Ret (old, r)
-    | SetVar x v => Ret (alist_add _ x v old, tt)
+    | GetVar x => '(_, r) <- unwrapU (alist_find _ x le) ;; Ret (le, r)
+    | SetVar x v =>
+      '(t, _) <- unwrapU (alist_find _ x le) ;;
+      if (has_type v t)
+      then Ret (alist_add _ x (t, v) le, tt)
+      else triggerUB
     end.
-
-(* Definition interp_imp `{Σ: GRA.t} {A} (t : itree (ImpState +' Es) A) : stateT fun_loc_env (itree Es) A := *)
-(*   let t' := interp (bimap handle_ImpState (id_ Es)) t in *)
-(*   interp_map t'. *)
 
 Definition interp_imp `{Σ: GRA.t} : itree (ImpState +' Es) ~> stateT lenv (itree Es) :=
   State.interp_state (case_ handle_ImpState ModSem.pure_state).
 
+Fixpoint init_lenv vts : lenv :=
+  match vts with
+  | [] => []
+  | (x, ty) :: t => (x, (ty, Vundef)) :: (init_lenv t)
+  end
+.
 
-(* Definition eval_imp `{Σ: GRA.t} (f: function) (args: list val) : itree Es val := *)
-(*   if (List.length f.(params) =? List.length args)%nat *)
-(*   then '(_, retv) <- (interp_imp (denote_stmt f.(body)) (List.combine f.(params) args));; Ret retv *)
-(*   else triggerUB. *)
+Fixpoint init_args params args (acc: lenv) : option lenv :=
+  match params, args with
+  | [], [] => Some acc
+  | (x, ty) :: pt, argv :: argt =>
+    if (has_type argv ty)
+    then (init_args pt argt (alist_add _ x (ty, argv) acc))
+    else None
+  | _, _ => None
+  end
+.
 
 Definition eval_imp `{Σ: GRA.t} (f: function) (args: list val) : itree Es val :=
-  if (List.length f.(params) =? List.length args)%nat
-  then '(_, retv) <- (interp_imp (denote_stmt f.(body)) (List.combine f.(params) args));; Ret retv
-  else triggerUB.
+  match (init_args f.(fn_params) args (init_lenv f.(fn_vars))) with
+  | Some le =>
+    '(_, retv) <- (interp_imp (denote_stmt f.(fn_body)) le) ;; Ret retv
+  | None => triggerUB
+  end
+.
 
+(** module components *)
+Definition modFuns := list (gname * function).
+Definition modVars := list (gname * val).
 
-(* ========================================================================== *)
-(**
-Section InterpImpProperties.
-  (** We can lift the underlying equational theory on [itree]s to include new
-      equations for working with [interp_imp].
-
-      In particular, we have:
-         - [interp_imp] respects [≈]
-         - [interp_imp] commutes with [bind].
-
-      We could justify more equations than just the ones below.  For instance,
-      _Imp_ programs also respect a coarser notation of equivalence for the
-      [env] state.  We exploit this possibility to implement optimzations
-      at the _Asm_ level (see AsmOptimizations.v).
-   *)
-
-  Context {E': Type -> Type}.
-  Notation E := (ImpState +' E').
-
-  (** This interpreter is compatible with the equivalence-up-to-tau. *)
-  Global Instance eutt_interp_imp {R}:
-    Proper (@eutt E R R eq ==> eq ==> @eutt E' (prod (env) R) (prod _ R) eq)
-           interp_imp.
-  Proof.
-    repeat intro.
-    unfold interp_imp.
-    unfold interp_map.
-    rewrite H0. eapply eutt_interp_state_eq; auto.
-    rewrite H. reflexivity.
-  Qed.
-
-  (** [interp_imp] commutes with [bind]. *)
-  Lemma interp_imp_bind: forall {R S} (t: itree E R) (k: R -> itree E S) (g : env),
-      (interp_imp (ITree.bind t k) g)
-    ≅ (ITree.bind (interp_imp t g) (fun '(g',  x) => interp_imp (k x) g')).
-  Proof.
-    intros.
-    unfold interp_imp.
-    unfold interp_map.
-    repeat rewrite interp_bind.
-    repeat rewrite interp_state_bind.
-    apply eqit_bind. red. intros.
-    destruct a as [g'  x].
-    simpl.
-    reflexivity.
-    reflexivity.
-  Qed.
-
-End InterpImpProperties.
-
-**)
+(** Imp module *)
+Record module : Type := mk_module {
+  mod_vars : modVars;
+  mod_funs : modFuns;
+  mod_main : gname
+}.
 
 (**** ModSemL ****)
 Module ImpMod.
+<<<<<<< HEAD
 Section MODSEML.
+=======
+Section MODSEML.
+
+>>>>>>> 3b74b52 (upgraded imp)
   Context `{GRA: GRA.t}.
   Variable mn: mname.
-  Variable prog: program.
+  Variable m: module.
 
   Set Typeclasses Depth 5.
-  Instance Initial_void1 : @Initial (Type -> Type) IFun void1 := @elim_void1. (*** TODO: move to ITreelib ***)
+  (* Instance Initial_void1 : @Initial (Type -> Type) IFun void1 := @elim_void1. (*** TODO: move to ITreelib ***) *)
 
   Definition modsem: ModSem.t := {|
-    ModSem.fnsems := List.map (fun '(fn, st) => (fn, cfun (eval_imp st))) prog;
+<<<<<<< HEAD
+    ModSem.fnsems :=
+      List.map (fun '(fn, f) => (fn, cfun (eval_imp f))) m.(mod_funs);
     ModSem.mn := mn;
     ModSem.initial_mr := ε;
     ModSem.initial_st := tt↑;
+=======
+    ModSem.fnsems :=
+      List.map (fun '(fn, f) => (fn, cfun (eval_imp f))) m.(mod_funs);
+    ModSem.mn := mn;
+    ModSem.initial_mr := ε;
+    ModSem.initial_st := tt↑;
+>>>>>>> 3b74b52 (upgraded imp)
   |}.
 
   Definition get_mod: Mod.t := {|
     Mod.get_modsem := fun _ => modsem;
-    Mod.sk := List.map (fun '(fn, _) => (fn, Sk.Gfun)) prog;
+    Mod.sk :=
+      (List.map (fun '(vn, vv) => (vn, Sk.Gvar vv)) m.(mod_vars)) ++
+      (List.map (fun '(fn, _) => (fn, Sk.Gfun)) m.(mod_funs));
   |}.
 
 End MODSEML.
@@ -494,19 +452,30 @@ Section Example_Extract.
        "input"  =# "input" - 1%Z end#;;#
     "output".
 
-  Definition factorial_fundef : function :=
-    {| params := ["input"] ; body := factorial |}.
+  Definition factorial_fundef : function := {|
+    fn_return := Tint;
+    fn_params := [("input", Tint)];
+    fn_vars := [("output", Tint); ("input", Tint)];
+    fn_body := factorial
+  |}.
 
   Definition main : stmt :=
-    "result" :=# (Fun "factorial") [4%Z : expr] ;;#
+    "result" :=# (Fun "factorial" Tint) [4%Z : expr] ;;#
     "result".
 
-  Definition main_fundef : function :=
-    {| params := [] ; body := main |}.
+  Definition main_fundef : function := {|
+    fn_return := Tint;
+    fn_params := [];
+    fn_vars := [("result", Tint)];
+    fn_body := main
+  |}.
 
-  Definition ex_extract : program :=
-    [("factorial", factorial_fundef); ("main", main_fundef)].
-
+  Definition ex_extract : module := {|
+    mod_vars := [];
+    mod_funs := [("factorial", factorial_fundef); ("main", main_fundef)];
+    mod_main := "main"
+  |}.
+  
   Definition ex_prog: Mod.t := ImpMod.get_mod "Main" ex_extract.
 
   Definition imp_ex := ModSemL.initial_itr_no_check (ModL.enclose ex_prog).
@@ -563,8 +532,8 @@ Section PROOFS.
   Lemma interp_imp_GetVar
         st0 x
     :
-      interp_imp (trigger (GetVar x)) st0 =
-      r <- unwrapU (alist_find _ x st0);; tau;; Ret (st0, r).
+      (interp_imp (trigger (GetVar x)) st0 : itree Es (_ * val)) =
+      '(_, r) <- unwrapU (alist_find _ x st0);; tau;; Ret (st0, r).
   Proof.
     unfold interp_imp. grind.
   Qed.
@@ -573,9 +542,13 @@ Section PROOFS.
         st0 x v
     :
       interp_imp (trigger (SetVar x v)) st0 =
-      tau;; Ret (alist_add _ x v st0, tt).
+      '(t, _) <- unwrapU (alist_find _ x st0) ;;
+      if (has_type v t)
+      then tau;; Ret (alist_add _ x (t, v) st0, tt)
+      else triggerUB.
   Proof.
-    unfold interp_imp. grind.
+    unfold interp_imp. grind. unfold triggerUB.
+    destruct (has_type v t); grind.    
   Qed.
 
   Lemma interp_imp_Call
@@ -621,20 +594,17 @@ Section PROOFS.
   Qed.
 
   Lemma eval_imp_unfold
-        input params body
+        fret fparams fvars fbody args
     :
-       ` vret : val <- eval_imp {| params := params; body := body |} input ;;
-       Ret (vret↑)
-      =
-       ` vret : val <-
-       (if ((Datatypes.length params) =? (Datatypes.length input))%nat
-        then
-          ` x : lenv * val <-
-          interp_imp
-            (denote_stmt body)
-            (List.combine params input);;
-          (let (_, retv) := x in Ret retv)
-        else triggerUB);; Ret (vret↑).
+      ` vret : val <- eval_imp (mk_function fret fparams fvars fbody) args ;; Ret (vret↑)
+               =
+               ` vret : val <-
+                        (match init_args fparams args (init_lenv fvars) with
+                         | Some le =>
+                           ITree.bind (interp_imp (denote_stmt fbody) le)
+                                      (fun x_ : lenv * val => let (_, retv) := x_ in Ret retv)
+                         | None => triggerUB
+                         end) ;; Ret (vret↑).
   Proof. reflexivity. Qed.
 
 End PROOFS.
@@ -660,8 +630,8 @@ Ltac imp_red :=
     | While _ _ => rewrite denote_stmt_While
     | Skip => rewrite denote_stmt_Skip
     | CallFun _ _ _ => rewrite denote_stmt_CallFun
-    | Expr _ => rewrite denote_stmt_Expr
-    | Expr_coerce _ => rewrite denote_stmt_Expr
+    | Return _ => rewrite denote_stmt_Return
+    | Return_coerce _ => rewrite denote_stmt_Return
     | _ => fail
     end
 
