theories/Imp2Clight.v
@@ -1,7 +1,3 @@
-From compcert Require Import Clight.
-From compcert Require Import Memory.
-From compcert Require Import Ctypes.
-
 Require Import Coqlib.
 Require Import Universe.
 Require Import Skeleton.
@@ -9,7 +5,150 @@ Require Import PCM.
 Require Import STS Behavior.
 Require Import Any.
 Require Import ModSem.
-Require Import SimSTS.
-Require Import STSNorm.
 Require Import Imp.
 
+From compcert Require Import Clight.
+From compcert Require Import Integers.
+From compcert Require Import Ctypes.
+
+Import Int.
+
+Set Implicit Arguments.
+
+Section Compile.
+
+  Definition cast (nextID: AST.ident) := var -> option (AST.ident * type).
+  Definition empty : cast 1%positive := fun _ => None.
+
+  Definition update_cast {i} newKey newType (curr: cast i) : cast (Pos.succ i):=
+    fun key =>
+      if (String.string_dec key newKey) then (Some (i, newType))
+      else (curr key).
+
+  Hypothesis is_int :
+    forall (intval : Z),
+      ((Zneg xH) < intval < modulus)%Z.
+  
+  Let attr_bot : attr := {|
+    attr_volatile := false; attr_alignas := None;
+  |}.
+
+  Let canon_Tint :=
+    (Tint I32 Signed attr_bot).
+
+  (* Let canon_Tptr := *)
+  (*   (Tpointer canon_Tint attr_bot). *)
+  
+  Fixpoint compile_expr leCast expr : option Clight.expr :=
+    match expr with
+    | Var x =>
+      match (leCast x) with
+      | None => None
+      | Some (i, t) => Some (Etempvar i t)
+      end
+    | Lit v =>
+      match v with
+      | Vint z => Some (Econst_int (mkint z (is_int z)) canon_Tint)
+      | _ => None
+      end
+    | Plus a b =>
+      match (compile_expr leCast a), (compile_expr leCast b) with
+      | Some (Econst_int x t), Some (Econst_int y s) =>
+        Some (Ebinop Cop.Oadd (Econst_int x t) (Econst_int y s) canon_Tint)
+      | _, _ => None
+      end
+    | Minus a b =>
+      match (compile_expr leCast a), (compile_expr leCast b) with
+      | Some (Econst_int x t), Some (Econst_int y s) =>
+        Some (Ebinop Cop.Osub (Econst_int x t) (Econst_int y s) canon_Tint)
+      | _, _ => None
+      end
+    | Mult a b =>
+      match (compile_expr leCast a), (compile_expr leCast b) with
+      | Some (Econst_int x t), Some (Econst_int y s) =>
+        Some (Ebinop Cop.Omul (Econst_int x t) (Econst_int y s) canon_Tint)
+      | _, _ => None
+      end
+    end
+  .
+
+  Fixpoint compile_exprs leCast (exprs: list Imp.expr) : option (list Clight.expr) :=
+    match exprs with
+    | h :: t =>
+      match (compile_expr leCast h), (compile_exprs leCast t) with
+      | Some h', Some t' => Some (h' :: t')
+      | _, _ => None
+      end
+    | [] => Some []
+    end
+  .
+  
+  Fixpoint type_Imp_expr (leCast: string -> option (AST.ident * type)) expr : option type :=
+    match expr with
+    | Var x =>
+      match (leCast x) with
+      | None => None
+      | Some (_, t) => Some t
+      end
+    | Lit v =>
+      match v with
+      | Vint _ => Some canon_Tint
+      | _ => None
+      end
+    | Plus a b =>
+      match (type_Imp_expr leCast a), (type_Imp_expr leCast b) with
+      | Some (Tint _ _ _), Some (Tint _ _ _) => Some canon_Tint
+      | _, _ => None
+      end
+    | Minus a b =>
+      match (type_Imp_expr leCast a), (type_Imp_expr leCast b) with
+      | Some (Tint _ _ _), Some (Tint _ _ _) => Some canon_Tint
+      | _, _ => None
+      end
+    | Mult a b =>
+      match (type_Imp_expr leCast a), (type_Imp_expr leCast b) with
+      | Some (Tint _ _ _), Some (Tint _ _ _) => Some canon_Tint
+      | _, _ => None
+      end
+    end
+  .
+  
+  Fixpoint compile_stmt leCast stmt : option Clight.statement :=
+    match stmt with
+    | Assign x e =>
+      match (type_Imp_expr leCast e) with
+      | Some t => Some (Sset ((update_cast x t leCast) x) (compile_expr leCast e))
+      | _ => None
+      end
+    | Seq s1 s2 =>
+      match (compile_stmt leCast s1), (compile_stmt leCast s2) with
+      | Some cs1, Some cs2 => Some (Ssequence cs1 cs2)
+      | _ => None
+      end
+    | If cond sif selse =>
+      match (compile_expr leCast cond), (compile_stmt leCast sif), (compile_stmt leCast selse) with
+      | Some cc, Some cif, Some celse =>
+        Some (Sifthenelse cc cif celse)
+      | _ => None
+      end
+    | While cond body =>
+      match (compile_expr leCast cond), (compile_stmt leCast body) with
+      | Some cc, Some cb => Some (Swhile cc cb)
+      | _ => None
+      end
+    | Skip =>
+      Some Sskip
+    | CallFun x ftype args =>
+      match (leCast x), (compile_exprs leCast args) with
+      | Some (i, t), Some cargs =>
+        match ftype with
+        | Fun fn =>
+          Some (Scall (Some i) (compile_expr (Var fn)) cargs
+      
+    | Return r =>
+    end
+  .
+  
+
+
+End Compile.
